examples/nsl_auth.v
@@ -258,7 +258,7 @@ Lemma wp_init c lI v0 lR kI kR :
   channel c -∗
   cryptis_ctx -∗
   nsl_ctx lI lR -∗
-  public (TKey Seal kI) -∗
+  aenc_key kI -∗
   □ (compromised_key kI → ▷ False) -∗
   public (TKey Seal kR) -∗
   {{{ lI ↦ v0 }}}
@@ -269,7 +269,8 @@ Lemma wp_init c lI v0 lR kI kR :
         □ (□ (compromised_key kR → ▷ False) -∗ ▷ session lR kI kR sk)
       else True }}}.
 Proof.
-iIntros "#chan_c #ctx #ctx' #p_kI #s_kI #p_kR %Ψ !> Hl Hpost".
+iIntros "#chan_c #ctx #ctx' #aenc_kI #s_kI #p_kR %Ψ !> Hl Hpost".
+iPoseProof (aenc_key_public with "aenc_kI") as "?".
 rewrite /init. wp_pures. wp_bind (mk_nonce _).
 iApply (wp_mk_nonce (λ _, corrupt kI kR) (λ _, False)%I) => //.
 iIntros "%nI _ #m_nI #p_nI _ token".
@@ -300,7 +301,7 @@ Lemma wp_resp c lI lR v0 kR :
   channel c -∗
   cryptis_ctx -∗
   nsl_ctx lI lR -∗
-  public (TKey Seal kR) -∗
+  aenc_key kR -∗
   □ (compromised_key kR → ▷ False) -∗
   {{{ lR ↦ v0 }}}
     resp c #lR kR
@@ -312,7 +313,8 @@ Lemma wp_resp c lI lR v0 kR :
         □ (□ (compromised_key kI → ▷ False) -∗ ▷^2 session lI kI kR sk)
       else True }}}.
 Proof.
-iIntros "#chan_c #ctx #ctx' #p_kR #honR %Ψ !> Hl Hpost".
+iIntros "#chan_c #ctx #ctx' #aenc_kR #honR %Ψ !> Hl Hpost".
+iPoseProof (aenc_key_public with "aenc_kR") as "?".
 rewrite /resp. wp_pures. wp_apply wp_pkey.
 wp_pures. wp_apply wp_recv => //; iIntros (m1) "#Hm1".
 wp_adec m1; last protocol_failure.
@@ -397,9 +399,9 @@ case: kt epkR' ekt => // -> _.
 iApply (wp_par (λ v, ∃ a : option term, ⌜v = repr a⌝ ∗ _)%I
                (λ v, ∃ a : option (term * term), ⌜v = repr a⌝ ∗ _)%I
           with "[HlI] [HlR]").
-- iApply (wp_init with "[//] [//] [//] p_pkI [] p_pkR' [$]") => //.
+- iApply (wp_init with "[//] [//] [//] aenc_kI [] p_pkR' [$]") => //.
   iIntros "!> %a H". iExists a. iSplit; first done. iApply "H".
-- iApply (wp_resp with "[//] [//] [//] p_pkR [//] [HlR]") => //.
+- iApply (wp_resp with "[//] [//] [//] aenc_kR [//] [HlR]") => //.
   iIntros "!> %a H"; iExists a; iSplit; first done. iApply "H".
 iIntros (v1 v2) "[H1 H2]".
 iDestruct "H1" as (a) "[-> H1]".
