nsl.v
@@ -80,7 +80,7 @@ Lemma wp_nsl_init c kI kR :
   channel c -∗
   cryptis_ctx -∗
   pk_auth_ctx N -∗
-  public (TKey Seal kI) -∗
+  aenc_key kI -∗
   public (TKey Seal kR) -∗
   {{{ init_confirm kI kR }}}
     nsl_init c kI (TKey Seal kR)
@@ -104,7 +104,7 @@ Lemma wp_nsl_resp c kR :
   channel c -∗
   cryptis_ctx -∗
   pk_auth_ctx N -∗
-  public (TKey Seal kR) -∗
+  aenc_key kR -∗
   {{{ resp_confirm kR }}}
     nsl_resp c kR
   {{{ (res : option (term * term)), RET repr res;
